update

Lemmas.String.fst
@@ -2,17 +2,16 @@ module Lemmas.String
 
 module S = FStar.String
 
-val string_of_int_return_not_empty_string: (n:int) -> Lemma (ensures S.length (string_of_int n) > 0) [SMTPat (string_of_int n)]
-let string_of_int_return_not_empty_string = admit()
+val string_of_int_return_not_empty_string: (n:int) -> Lemma (ensures S.length (string_of_int n) > 0 /\ (string_of_int n) <> "") [SMTPat (string_of_int n)]
 
 val strcat_add_length: (s1:string) -> (s2:string) -> Lemma (ensures (S.length s1) + (S.length s2) = (S.length (s1 ^ s2))) [SMTPat (s1 ^ s2)]
-let strcat_add_length = admit()
 
 val string_length_is_nat: (s:string) -> Lemma (S.length s >= 0)
-let string_length_is_nat = admit()
 
 val empty_string_length_is_zero: (s:string) -> Lemma (requires s = "") (ensures S.length s = 0)
-let empty_string_length_is_zero = admit()
+
+val zero_length_string_is_empty: (s:string) -> Lemma (requires S.length s = 0) (ensures s = "")
 
 val not_empty_string_length_is_pos: (s:string) -> Lemma (requires s <> "") (ensures S.length s > 0)
-let not_empty_string_length_is_pos = admit()
+
+val pos_length_string_is_not_empty: (s:string) -> Lemma (requires S.length s > 0) (ensures s <> "")
